Compiler/UnverifiedIncompleteCompiler.v
@@ -1,4 +1,3 @@
-Require Import Coq.ZArith.BinIntDef Coq.ZArith.BinInt Coq.ZArith.Zdiv.
 Require Import Kami.Syntax Kami.Notations RecordUpdate.RecordSet Kami.Compiler.Rtl Kami.StateMonad.
 
 
@@ -295,7 +294,7 @@ Definition getRegInit (y: sigT RegInitValT): {x: Kind & option (ConstT x)} :=
                                                        | _ => Void
                                                        end with
                 | SyntaxConst k c => c
-                | _ => (zToWord 0 0)
+                | _ => (ZToWord 0 0)
                 end
          end.
 
