Lib/HexNotationWord.v
@@ -1,33 +1,31 @@
 Require Export Kami.Lib.Word.
 Require Export Kami.Lib.HexNotation.
 Open Scope word_scope.
-Require Import Coq.ZArith.BinIntDef Coq.ZArith.BinInt Coq.ZArith.Zdiv.
-
 
 Notation "'Ox' a" := (NToWord _ (hex a)) (at level 50).
 
 Notation "sz ''h' a" := (NToWord sz (hex a)) (at level 50).
 
-Goal 8'h"a" = zToWord 8 (wordVal _ (NToWord 4 10)).
+Goal 8'h"a" = ZToWord 8 (wordVal _ (NToWord 4 10)).
 Proof.
   reflexivity.
 Qed.
 
-Goal Ox"41" = zToWord 7 65.
+Goal Ox"41" = ZToWord 7 65.
 Proof.
   reflexivity.
 Qed.
 
-Notation "sz ''b' a" := (zToWord sz (Z.of_nat (bin a))) (at level 50).
+Notation "sz ''b' a" := (ZToWord sz (Z.of_nat (bin a))) (at level 50).
 
-Notation "''b' a" := (zToWord _ (Z.of_nat (bin a))) (at level 50).
+Notation "''b' a" := (ZToWord _ (Z.of_nat (bin a))) (at level 50).
 
-Goal 'b"00001010" = zToWord 8 (wordVal _ (NToWord 4 10)).
+Goal 'b"00001010" = ZToWord 8 (wordVal _ (NToWord 4 10)).
 Proof.
   reflexivity.
 Qed.
 
-Goal 'b"1000001" = zToWord 7 65.
+Goal 'b"1000001" = ZToWord 7 65.
 Proof.
   reflexivity.
 Qed.
