PProperties.v
@@ -4,7 +4,6 @@ Import ListNotations.
 Require Import Coq.Sorting.Permutation.
 Require Import Coq.Sorting.PermutEq.
 Require Import RelationClasses Setoid Morphisms.
-Require Import ZArith.
 
 Lemma PSemAction_SemAction o k:
   forall (a : ActionT type k) (readRegs newRegs : RegsT) (calls : MethsT) (fret : type k),
