SyntaxDoubleWrites.v
@@ -4,7 +4,6 @@ Require Export Kami.Lib.Word Kami.Lib.VectorFacts Kami.Lib.EclecticLib Kami.AllN
 Export Word.Notations.
 
 Require Import Permutation RecordUpdate.RecordSet.
-Require Import ZArith.
 Import ListNotations.
 
 Global Set Implicit Arguments.
